Add a notion of oracles, so we can talk about SUPERHALT

main.v
@@ -1,31 +1,54 @@
 (*could parametrize by what is currently bool for more diverse return types*)
 
 (** Definition of a machine, and some machines.*)
-CoInductive machine :=
-| Halts : bool -> machine
-| Steps : machine -> machine
+CoInductive oracle_machine {i o} :=
+| Halts : bool -> oracle_machine
+| Steps : oracle_machine -> oracle_machine
+| Calls : i -> (o -> oracle_machine) -> oracle_machine
 .
 
+
+Definition machine := @oracle_machine Empty_set Empty_set.
+
+
+(* The eval_machine proposition asserts that a machine halts with output bool b. *)
+Inductive eval_oracle_machine {i o} (oracle: i -> o -> Prop) : @oracle_machine i o -> bool -> Prop :=
+| EvalHalts b :
+    eval_oracle_machine oracle (Halts b) b
+| EvalSteps m b :
+    eval_oracle_machine oracle m b ->
+    eval_oracle_machine oracle (Steps m) b
+| EvalCalls input output continuation b :
+    oracle input output ->
+    eval_oracle_machine oracle (continuation output) b -> 
+    eval_oracle_machine oracle (Calls input continuation) b
+.
+
+Definition eval_tm : machine -> bool -> Prop := eval_oracle_machine (fun i => fun o => True). 
+
+
+(* Some simple Turing machines: looper, collatz, dumb. *)
 CoFixpoint looper : machine := Steps looper.
 
-CoFixpoint collatz (x:nat) :machine :=
-  if (true)
-  then if (true)
-       then Steps (collatz x)
-       else Steps (collatz (3*x+1))
-  else Halts true.
+Require Import Nat.
 
-Definition dumb (b:bool) : machine := Halts b.
+CoFixpoint collatz (x:nat) :machine :=
+  if leb x 1
+  then Halts true
+  else if even x
+       then Steps (collatz (div2 x))
+       else Steps (collatz (3*x+1))
+.
+
+Definition halter (b:bool) : machine := Halts b.
 
 
 (** Definition of a language, and some languages.*)
 Definition language input := input -> Prop.
 
-Inductive eval_tm : machine -> bool -> Prop :=
-| EvalHalts b : eval_tm (Halts b) b
-| EvalSteps m b : eval_tm m b -> eval_tm (Steps m) b.
-
 Definition halt_tm : language machine := fun m => exists b, eval_tm m b.
+
+Definition superhalt_tm : language oracle_machine := fun om => exists b, eval_oracle_machine (fun i : machine => fun o : bool => eval_tm i o) om b.
 
 Definition a_tm : language machine := fun m => eval_tm m true.
 
@@ -42,14 +65,14 @@ Definition decidable {input} (l : language input) : Prop :=
   exists (im : input -> machine),
     decides im l.
 
-Hint Constructors eval_tm.
+Hint Constructors eval_oracle_machine.
 
-Theorem dumb_decides_l_true: decides dumb (l_true).
+Theorem halter_decides_l_true: decides halter (l_true).
 Proof.
   intro i.
   exists i.
   split.
-  auto.
+  constructor.
   unfold l_true.
   firstorder.
 Qed.
@@ -105,6 +128,7 @@ Definition frob (m : machine) : machine :=
   match m with
     | Halts b => Halts b
     | Steps m' => Steps m'
+    | Calls input continuation => Calls input continuation
   end.
 
 Lemma frob_eq m : m = frob m.
@@ -117,6 +141,7 @@ CoFixpoint invert_output (m: machine): machine :=
     | Halts true => looper
     | Halts false => Halts true
     | Steps m => Steps (invert_output m)
+    | Calls input continuation => Calls input (fun output => invert_output (continuation output))
   end.
 
 Lemma looper_loops :
@@ -129,6 +154,7 @@ Proof.
   - injection Heqm.
     rewrite (frob_eq looper).
     assumption.
+  - discriminate.
 Qed.
 
 Lemma invert_output_lemma:
@@ -142,13 +168,14 @@ Proof.
     exists true.
     rewrite (frob_eq (invert_output _)).
     apply EvalHalts.
-    destruct IHeval_tm.
+    destruct IHeval_oracle_machine.
     reflexivity.
     exists x.
     rewrite (frob_eq (invert_output _)).
     simpl.
     apply EvalSteps.
-    assumption. }
+    assumption.
+    destruct input. }
   { destruct 1.
     remember (invert_output m).
     rewrite (frob_eq (invert_output _)) in Heqm0.
@@ -160,9 +187,10 @@ Proof.
         { apply EvalHalts. }
       }
       { discriminate. }
+      { destruct e. }
     }
     { destruct m0.
-      { apply IHeval_tm.
+      { apply IHeval_oracle_machine.
         destruct b0.
         { injection Heqm0.
           intro.
@@ -172,11 +200,13 @@ Proof.
       { injection Heqm0.
         intro.
         constructor.
-        apply IHeval_tm.
+        apply IHeval_oracle_machine.
         rewrite <- frob_eq.
         assumption.
       }
+      { destruct e. }
     }
+    { destruct input. }
   }
 Qed.
 
@@ -191,8 +221,9 @@ Proof.
   reflexivity.
   inversion 1.
   subst.
-  apply IHeval_tm.
+  apply IHeval_oracle_machine.
   assumption.
+  destruct input.
 Qed.
   
   
@@ -223,7 +254,7 @@ Proof.
   destruct x.
   { eapply only_one_value.
     { apply <- H2.
-      destruct (proj2 H0 eq_refl).
+      destruct (proj2 H0 eq_refl).
       exists x.
       apply H1.
       assumption. }
@@ -237,6 +268,21 @@ Proof.
 Qed.
 
            
-Definition atm_undecidable: (undecidable atm).
+(*Definition atm_undecidable: (undecidable atm).*)
+
+
+Theorem superhalting_problem_undecidable: undecidable superhalt_tm.
+Proof.
+
+
+
+
+
+
+
+
+
+Theorem l_leq_superhalt
+
 
 (*whatever!*)
